sparse/spec_sparse.v
@@ -23,6 +23,52 @@ Definition crs_rep (sh: share) (mval: matrix Tdouble) (p: val) : mpred :=
   data_at sh (tarray tuint (Zlength col_ind)) (map Vint (map Int.repr col_ind)) ci *
   data_at sh (tarray tuint (matrix_rows mval + 1)) (map Vint (map Int.repr row_ptr)) rp.
 
+Definition crs_row_vector_multiply_spec :=
+ DECLARE _crs_row_vector_multiply
+ WITH sh1: share, sh2: share, sh3: share,
+      m: val, mval: matrix Tdouble, v: val, vval: vector Tdouble, i: Z
+ PRE [ tptr t_crs, tptr tdouble, tuint ]
+    PROP(readable_share sh1; readable_share sh2; writable_share sh3;
+             matrix_cols mval (Zlength vval);
+             matrix_rows mval < Int.max_unsigned;
+             Zlength vval < Int.max_unsigned;
+             0 <= i < matrix_rows mval;
+             Forall finite vval;
+             Forall (Forall finite) mval)
+    PARAMS(m; v; Vint (Int.repr i))
+    SEP (crs_rep sh1 mval m;
+         data_at sh2 (tarray tdouble (Zlength vval)) (map Vfloat vval) v)
+ POST [ tdouble ]
+   EX s: ftype Tdouble,
+    PROP(float_eqv s (dotprod (Znth i mval) vval)) 
+    RETURN(Vfloat s)
+    SEP (crs_rep sh1 mval m;
+          data_at sh2 (tarray tdouble (Zlength vval)) (map Vfloat vval) v).
+
+Definition crs_matrix_vector_multiply_byrows_spec :=
+ DECLARE _crs_matrix_vector_multiply_byrows
+ WITH sh1: share, sh2: share, sh3: share,
+      m: val, mval: matrix Tdouble, v: val, vval: vector Tdouble, p: val
+ PRE [ tptr t_crs, tptr tdouble, tptr tdouble ]
+    PROP(readable_share sh1; readable_share sh2; writable_share sh3;
+             matrix_cols mval (Zlength vval);
+             matrix_rows mval < Int.max_unsigned;
+             Zlength vval < Int.max_unsigned;
+             Forall finite vval;
+             Forall (Forall finite) mval)
+    PARAMS(m; v; p)
+    SEP (crs_rep sh1 mval m;
+         data_at sh2 (tarray tdouble (Zlength vval)) (map Vfloat vval) v; 
+         data_at_ sh3 (tarray tdouble (matrix_rows mval)) p)
+ POST [ tvoid ]
+   EX result: vector Tdouble,
+    PROP(floatlist_eqv result (matrix_vector_mult mval vval)) 
+    RETURN()
+    SEP (crs_rep sh1 mval m;
+          data_at sh2 (tarray tdouble (Zlength vval)) (map Vfloat vval) v; 
+          data_at sh3 (tarray tdouble (matrix_rows mval)) 
+             (map Vfloat result) p).
+
 Definition crs_matrix_vector_multiply_spec :=
  DECLARE _crs_matrix_vector_multiply
  WITH sh1: share, sh2: share, sh3: share,
@@ -47,4 +93,7 @@ Definition crs_matrix_vector_multiply_spec :=
           data_at sh3 (tarray tdouble (matrix_rows mval)) 
              (map Vfloat result) p).
 
-Definition SparseASI : funspecs := [ crs_matrix_vector_multiply_spec ].
+Definition SparseASI : funspecs := [ 
+   crs_row_vector_multiply_spec;
+   crs_matrix_vector_multiply_byrows_spec;
+   crs_matrix_vector_multiply_spec ].
