sparse/verif_sparse_byrows.v
@@ -1,0 +1,182 @@
+Require Import VST.floyd.proofauto.
+Require Import Iterative.floatlib.
+From Iterative.sparse Require Import sparse sparse_model spec_sparse.
+Require Import vcfloat.VCFloat.
+Require Import vcfloat.FPCompCert.
+Require Import VSTlib.spec_math.
+
+Set Bullet Behavior "Strict Subproofs".
+
+Open Scope logic.
+
+Definition Gprog: funspecs := SparseASI ++ MathASI.
+
+Lemma body_crs_row_vector_multiply: semax_body Vprog Gprog f_crs_row_vector_multiply crs_row_vector_multiply_spec.
+Proof.
+start_function.
+rename H3 into FINmval.
+assert (0 <= matrix_rows mval) by (unfold matrix_rows; rep_lia).
+forward.
+forward.
+forward.
+freeze FR1 := (data_at sh1 _ _ _).
+rename v0 into vp.
+assert_PROP (0 <= i + 1 < Zlength row_ptr)
+  by (entailer!; list_solve).
+forward.
+forward.
+clear H6.
+assert (CRS := H5).
+assert (COLS := crs_rep_matrix_cols _ _ _ _ _ H5).
+destruct H5 as [H2' [H7 [H8 [H9 H10]]]].
+ assert_PROP (0 <= i < Zlength row_ptr - 1)
+  by (entailer!; list_solve).
+forward_for_simple_bound (Znth (i + 1) row_ptr)
+  (EX h:Z, PROP(0 <= Znth i row_ptr <= h)
+   LOCAL (
+   temp _s (Vfloat (partial_row i h vals col_ind row_ptr vval));
+   temp _i (Vint (Int.repr i));
+   temp _hi (Vint (Int.repr (Znth (i+1) row_ptr))); 
+   temp _row_ptr rp; temp _col_ind ci; temp _val vp;
+   temp _m m; temp _v v)
+   SEP (FRZL FR1;
+   data_at sh1 (tarray tdouble (Zlength col_ind)) (map Vfloat vals) vp;
+   data_at sh1 (tarray tuint (Zlength col_ind))
+     (map Vint (map Int.repr col_ind)) ci;
+   data_at sh1 (tarray tuint (matrix_rows mval + 1))
+     (map Vint (map Int.repr row_ptr)) rp;
+   data_at sh2 (tarray tdouble (Zlength vval)) (map Vfloat vval) v))%assert.
+-
+ clear - H9 H2 H2'. unfold matrix_rows in H2.  list_solve.
+-
+ forward.
+change float with (ftype Tdouble) in *. 
+ EExists. entailer!.
+ split3. 
+ clear - H9 H5. list_solve. 
+ clear - H9 H5. list_solve.
+ f_equal. erewrite partial_row_start. reflexivity. eassumption.
+-
+rename i0 into h.
+assert (h <= Int.max_unsigned). clear - H9 H6 H5. list_solve.
+forward. apply prop_right. list_solve.
+progress change float with (ftype Tdouble) in *. 
+entailer!.
+rewrite Znth_map. hnf; auto.
+clear - H6 H7 H5 H2 H2' H9. unfold matrix_rows in *. list_solve.
+assert  (0 <= h < Zlength col_ind).
+  rewrite H8.  clear - H5 H2' H9 H6. list_solve.
+forward.
+progress change float with (ftype Tdouble) in *. 
+assert (0 <= Znth h col_ind < Zlength vval). {
+     assert (Znth i row_ptr <= h < Znth (i+1) row_ptr) by lia.
+     assert (Znth (i+1) row_ptr <= Zlength col_ind) by list_solve.
+     clear - COLS H H14 H6 H2 H10 H12 H15.
+      replace (Znth h col_ind) with 
+              (Znth (h-Znth i row_ptr) (sublist (Znth i row_ptr) (Znth (i+1) row_ptr) col_ind))
+         by list_solve.
+     specialize (H10 _ H2).
+    pose proof (crs_row_rep_col_range _ _ _ _ H10).
+    specialize (H0 (h - Znth i row_ptr)).
+    autorewrite with sublist in H0. autorewrite with sublist. 
+  rewrite <- (sublist.Forall_Znth _ _ _ H2 H), (sublist.Forall_Znth _ _ _ H2 COLS).
+  apply H0. list_solve.
+  }
+forward.
+  change float with (ftype Tdouble) in *.
+  rewrite (@Znth_map (ftype Tdouble) _ _ _ h Vfloat) by rep_lia.
+  rewrite (@Znth_map (ftype Tdouble) _ _ _ (Znth h col_ind)) by rep_lia.
+  forward_call (Znth h vals, Znth (Znth h col_ind) vval, partial_row i h vals col_ind row_ptr vval).
+  forward.
+  entailer!.
+  f_equal.
+  change (Binary.Bfma _ _ _ _ _ _ _ _ _) with 
+   (@BFMA _ Tdouble (Znth h vals) (Znth (Znth h col_ind) vval)
+     (partial_row i h vals col_ind row_ptr vval)
+  ).
+  eapply partial_row_next; try eassumption; lia.
+-
+ forward.
+ Exists  (partial_row i (Znth (i + 1) row_ptr) vals col_ind row_ptr vval).
+ entailer!.
+ erewrite partial_row_end; try eassumption.
+ unfold matrix_vector_mult.
+ rewrite Znth_map by rep_lia. reflexivity.
+  rewrite <- (sublist.Forall_Znth _ _ _ H2 H), (sublist.Forall_Znth _ _ _ H2 COLS); auto.
+ unfold crs_rep.
+ thaw FR1.
+ Exists vp ci rp cols vals col_ind row_ptr.
+ entailer!.
+Qed.
+
+Lemma fold_crs_rep:
+  forall sh  (p v ci rp: val) mval cols (vals: list (ftype Tdouble))  col_ind row_ptr,
+     crs_rep_aux mval cols vals col_ind row_ptr ->
+     data_at sh t_crs
+          (v, (ci, (rp, (Vint (Int.repr (matrix_rows mval)),
+                      Vint (Int.repr cols))))) p *
+     data_at sh (tarray tdouble (Zlength col_ind)) (map Vfloat vals) v *
+     data_at sh (tarray tuint (Zlength col_ind))
+                     (map Vint (map Int.repr col_ind)) ci *
+     data_at sh (tarray tuint (matrix_rows mval + 1))
+            (map Vint (map Int.repr row_ptr)) rp
+     |-- crs_rep sh mval p.
+Proof.
+intros.
+unfold crs_rep.
+Exists v ci rp cols vals col_ind row_ptr.
+rewrite prop_true_andp by auto.
+cancel.
+Qed.
+
+
+Lemma body_crs_matrix_vector_multiply_byrows: semax_body Vprog Gprog f_crs_matrix_vector_multiply_byrows crs_matrix_vector_multiply_byrows_spec.
+Proof.
+start_function.
+forward.
+sep_apply fold_crs_rep. clear H4 v0 ci rp vals col_ind row_ptr cols.
+forward_for_simple_bound (Zlength mval)
+  (EX i:Z, EX result: list (ftype Tdouble),
+   PROP(floatlist_eqv result (sublist 0 i (matrix_vector_mult mval vval))) 
+   LOCAL (temp _rows (Vint (Int.repr (matrix_rows mval))); 
+   temp _m m; temp _v v; temp _p p)
+   SEP (crs_rep sh1 mval m;
+   data_at sh2 (tarray tdouble (Zlength vval)) (map Vfloat vval) v;
+   data_at sh3 (tarray tdouble (matrix_rows mval)) 
+      (map Vfloat result ++ Zrepeat Vundef (matrix_rows mval - i)) p))%assert.
+- unfold matrix_rows in H0; lia.
+- Exists (@nil (ftype Tdouble)). simpl app. entailer!.
+    rewrite sublist_nil. constructor.
+     apply derives_refl.
+- forward_call (sh1,sh2,sh3, m, mval, v, vval, i).
+   Intros s.
+   unfold matrix_rows in H0.
+   forward.
+   progress change float with (ftype Tdouble) in *. 
+   Exists (result ++ [s]).
+   entailer!. 
+   clear H11 H12 H10 H9 H8 H7 PNp PNv PNm.
+   assert (Zlength (matrix_vector_mult mval vval) = Zlength mval). 
+      unfold matrix_vector_mult. list_solve.
+   rewrite (sublist_split 0 i (i+1)) by list_solve.
+   apply Forall2_app.
+   auto.
+   rewrite sublist_len_1 by rep_lia.
+   constructor; [ | constructor].
+   unfold matrix_vector_mult. rewrite Znth_map by rep_lia. auto.
+   assert (Zlength result = i). {
+     clear - H5 H4. unfold matrix_vector_mult in H5.
+      apply Forall2_Zlength in H5. rewrite H5.
+    list_solve.
+   }
+   apply derives_refl'; f_equal.
+   unfold matrix_rows; subst i. clear H9 H11 H12 H10 H8 H7 PNp PNv PNm H5.
+    list_solve.
+-
+ Intro result. Exists result.
+ unfold matrix_rows in *. list_simplify.
+ entailer!.
+ unfold matrix_vector_mult in H8 |- *.
+ rewrite sublist_same in H8 by list_solve. auto.
+Qed.
+
